

8. $\dfrac{d (\cot x)}{dx} = -\csc^2 x$

9. $\dfrac{d (\sec x)}{dx} = \sec x \cdot \tan x$

10. $\dfrac{d (\csc x)}{dx} = -\csc x \cdot \cot x$

11. $f(x) = e^x$
\begin{align*}
    f'(x) &= \lim_{\Delta x \to 0} \dfrac{f(x+\Delta x) - f(x)}{\Delta x} \\
    &= \lim_{\Delta x \to 0} \dfrac{e^{x+\Delta x} - e^x}{\Delta x} \\
    &= \lim_{\Delta x \to 0} \dfrac{e^x \left(e^{\Delta x} - 1\right)}{\Delta x} \\
    &= \lim_{\Delta x \to 0} \dfrac{e^x \left[1 + \Delta x + \dfrac{(\Delta x)^2}{2!} + \dotsb - 1\right]}{\Delta x} \\
    &= \lim_{\Delta x \to 0} \dfrac{e^x \left(\Delta x + \dfrac{(\Delta x)^2}{2!} + \cdots \right)}{\Delta x} \\
    &= \lim_{\Delta x \to 0} \left( e^x \left[1 + \dfrac{\Delta x}{2!} + \dotsb \right] \right) = e^x
\end{align*}

12. $f(x) = \ln x$
\begin{align*}
    f'(x) &= \lim_{\Delta x \to 0} \dfrac{f(x+\Delta x) - f(x)}{\Delta x} \\
    &= \lim_{\Delta x \to 0} \dfrac{\ln (x+\Delta x) - \ln x}{\Delta x} \\
    &= \lim_{\Delta x \to 0} \dfrac{\ln x \left( 1 + \dfrac{\Delta x}{x} \right) - \ln x}{\Delta x} \\
    &= \lim_{\Delta x \to 0} \dfrac{\ln\left( 1 + \dfrac{\Delta x}{x} \right)}{\Delta x} \\
    &= \lim_{\Delta x \to 0} \left( \dfrac{\Delta x}{x} - \dfrac{1}{2} \left( \dfrac{\Delta x}{x} \right)^2 
    + \dfrac{1}{3} \left( \dfrac{\Delta x}{x} \right)^3 - \cdots \right) \dfrac{1}{\Delta x} \\
    &= \lim_{\Delta x \to 0} \left( \dfrac{1}{x} - \dfrac{1}{2} \dfrac{\Delta x}{x^2} 
    + \dfrac{1}{3} \dfrac{(\Delta x)^2}{x^3} - \cdots \right) \\
    &= \dfrac{1}{x}
\end{align*}

13. $f(x) = \sin^{-1} x$
\begin{align*}
    f'(x) &= \lim_{\Delta x \to 0} \dfrac{f(x+\Delta x) - f(x)}{\Delta x} = \lim_{\Delta x \to 0} 
    \dfrac{\sin^{-1} (x + \Delta x) - \sin^{-1} x}{\Delta x}
\end{align*}

