

\subsection*{Differential Coefficient (or Derivative)}

Differential coefficient or derivative of a function \( f(x) \) with respect to \( x \), denoted by \( f'(x) \), is defined as
\begin{align*}
    f'(x) &= \lim_{h \to 0} \frac{f(x + h) - f(x)}{h}
\end{align*}

Let 
\[
y = f(x)
\]

\[
y + \Delta y = f(x + \Delta x)
\]

\begin{align*}
    \therefore \quad \lim_{\Delta x \to 0} \frac{\Delta y}{\Delta x} &= \lim_{\Delta x \to 0} \frac{f(x + \Delta x) - f(x)}{\Delta x} = f'(x)
\end{align*}

\begin{align*}
    \lim_{\Delta x \to 0} \frac{\Delta y}{\Delta x} \intertext{is denoted by} \frac{dy}{dx}
\end{align*}

Thus,
\begin{align*}
    \frac{dy}{dx} &= f'(x)
\end{align*}

\( f'(x) \) and \( \frac{d \left( f(x) \right)}{dx} \), both denote derivative of \( f(x) \) with respect to \( x \).

\subsection*{Differential Coefficients of Some Functions}

\begin{enumerate}
    \item \( f(x) = c \) (constant)
        \begin{align*}
            f'(x) &= \lim_{\Delta x \to 0} \frac{f(x + \Delta x) - f(x)}{\Delta x} \\
                &= \lim_{\Delta x \to 0} \frac{c - c}{\Delta x} = \lim_{\Delta x \to 0} \frac{0}{\Delta x} = 0.
        \end{align*}
    \item \( f(x) = x \)
        \begin{align*}
            f'(x) &= \lim_{\Delta x \to 0} \frac{f(x + \Delta x) - f(x)}{\Delta x} \\
                &= \lim_{\Delta x \to 0} \frac{(x + \Delta x) - x}{\Delta x} \\
                &= \lim_{\Delta x \to 0} \frac{\Delta x}{\Delta x} = 1.
        \end{align*}

    \item \( f(x) = x^2 \)
        \begin{align*}
            f'(x) &= \lim_{\Delta x \to 0} \frac{f(x + \Delta x) - f(x)}{\Delta x}\\
            &= \lim_{\Delta x \to 0} \frac{(x + \Delta x)^2 - x^2}{\Delta x} \\
            &= \lim_{\Delta x \to 0} \frac{2x \cdot \Delta x + (\Delta x)^2}{\Delta x} \\
            &= \lim_{\Delta x \to 0} \frac{2x + \Delta x}{\Delta x} = 2x 
        \end{align*}


    \item $f(x) = x^n$, $n$ is a rational number.
        \begin{align*}
            f'(x) &= \lim_{\Delta x \to 0} \frac{f(x + \Delta x) - f(x)}{\Delta x} \\
            &= \lim_{\Delta x \to 0} \frac{(x + \Delta x)^n - x^n}{\Delta x} \\
            &= x^n \lim_{\Delta x \to 0} \frac{\left(1 + \frac{\Delta x}{x}\right)^n - 1}{\Delta x} \\
            &= x^n \lim_{\Delta x \to 0} \frac{ \left[ 1 + n \left(\frac{\Delta x}{x}\right) + \frac{n(n-1)}{2!} \left(\frac{\Delta x}{x}\right)^2 + \cdots \right] - 1}{\Delta x} \\
            &= x^n \lim_{\Delta x \to 0} \frac{n}{x} \left[ \frac{\Delta x}{\Delta x} \right] \left(1 + \frac{n(n - 1)}{2!}\frac{\Delta x}{x} + \cdots\right) - 1 \\
            &= \lim_{ \Delta x \to 0} x^{n - 1} \left[ n \left( 1 + \frac{n(n-1)}{2!}\frac{\Delta x}{x} + \cdots\right) \right] = nx^{n - 1}
        \end{align*}

    \item $f(x) = \sin x$
        \begin{align*}
            f'(x) &= \lim_{\Delta x \to 0} \frac{f(x + \Delta x) - f(x)}{\Delta x} \\
            &= \lim_{\Delta x \to 0} \frac{\sin(x + \Delta x) - \sin x}{\Delta x} \\
            &= \lim_{\Delta x \to 0} \frac{2 \cos \left(x + \frac{\Delta x}{2}\right) \cdot \sin \left( \frac{\Delta x}{2}\right)}{\Delta x} \\
            &= \lim_{\Delta x \to 0} \cos \left(x + \frac{\Delta x}{2}\right) \cdot \frac{\sin \left( \frac{\Delta x}{2}\right)}{\frac{\Delta x}{2}} \\
            &= \cos x \cdot 1 = \cos x
        \end{align*}
            Similarly, we can prove following five results (6, 7, 8, 9, and 10).
    
    \item $\frac{d(\cos x)}{dx} = -\sin x $
    \item $\frac{d(\tan x)}{dx} = \sec^2 x$
    \item $\dfrac{d (\cot x)}{dx} = -\cosec^2 x$

    \item $\dfrac{d (\sec x)}{dx} = \sec x \cdot \tan x$
        
    \item $\dfrac{d (\csc x)}{dx} = -\cosec x \cdot \cot x$
        
    \item $f(x) = e^x$
        \begin{align*}
            f'(x) &= \lim_{\Delta x \to 0} \dfrac{f(x+\Delta x) - f(x)}{\Delta x} \\
            &= \lim_{\Delta x \to 0} \dfrac{e^{x+\Delta x} - e^x}{\Delta x} \\
            &= \lim_{\Delta x \to 0} \dfrac{e^x \left(e^{\Delta x} - 1\right)}{\Delta x} \\
            &= \lim_{\Delta x \to 0} \dfrac{e^x \left[1 + \Delta x + \dfrac{(\Delta x)^2}{2!} + \dotsb - 1\right]}{\Delta x} \\
            &= \lim_{\Delta x \to 0} \dfrac{e^x \left(\Delta x + \dfrac{(\Delta x)^2}{2!} + \cdots \right)}{\Delta x} \\
            &= \lim_{\Delta x \to 0} \left( e^x \left[1 + \dfrac{\Delta x}{2!} + \dotsb \right] \right) = e^x
        \end{align*}
        
    \item $f(x) = \ln x$
        \begin{align*}
            f'(x) &= \lim_{\Delta x \to 0} \dfrac{f(x+\Delta x) - f(x)}{\Delta x} \\
            &= \lim_{\Delta x \to 0} \dfrac{\ln (x+\Delta x) - \ln x}{\Delta x} \\
            &= \lim_{\Delta x \to 0} \dfrac{\ln x \left( 1 + \dfrac{\Delta x}{x} \right) - \ln x}{\Delta x} \\
            &= \lim_{\Delta x \to 0} \dfrac{\ln\left( 1 + \dfrac{\Delta x}{x} \right)}{\Delta x} \\
            &= \lim_{\Delta x \to 0} \left( \dfrac{\Delta x}{x} - \dfrac{1}{2} \left( \dfrac{\Delta x}{x} \right)^2 
            + \dfrac{1}{3} \left( \dfrac{\Delta x}{x} \right)^3 - \cdots \right) \dfrac{1}{\Delta x} \\
            &= \lim_{\Delta x \to 0} \left( \dfrac{1}{x} - \dfrac{1}{2} \dfrac{\Delta x}{x^2} 
            + \dfrac{1}{3} \dfrac{(\Delta x)^2}{x^3} - \cdots \right) \\
            &= \dfrac{1}{x}
        \end{align*}
        
    \item $f(x) = \sin^{-1} x$
        \begin{align*}
            f'(x) &= \lim_{\Delta x \to 0} \dfrac{f(x+\Delta x) - f(x)}{\Delta x}\\
            &= \lim_{\Delta x \to 0} \dfrac{\sin^{-1} (x + \Delta x) - \sin^{-1} x}{\Delta x}\\
            \intertext{Let $\sin^{-1} x = y$}
            \intertext{and}
            \sin^{-1}(x + \Delta x) = y + \Delta y\\
            \intertext{$\therefore \sin y = x$}
            \sin(y + \Delta y) &= x + \Delta x\\
            \therefore \Delta x &= \sin(y + \Delta y) - \sin y\\
            \intertext{As $\Delta x \to 0$, $\Delta y \to 0$}
            \intertext{On substitution,}
            f'(x) &= \lim_{\Delta x \to 0} \frac{\sin^{-1}(x + \Delta x) - \sin^{-1} x}{\Delta x} \\
            &= \lim_{\Delta y \to 0} \frac{(y + \Delta y) - y}{\sin(y + \Delta y) - \sin y} \\
            &= \lim_{\Delta y \to 0} \frac{\Delta y}{2 \cos \left( y + \frac{\Delta y}{2} \right) \cdot \sin \left( \frac{\Delta y}{2} \right)} \\
            &= \lim_{\Delta y \to 0} \frac{1}{\cos \left( y + \frac{\Delta y}{2} \right) \cdot \sin \left( \frac{\Delta y}{2} \right)} \cdot \frac{\Delta y}{2} \\
            &= \frac{1}{\cos y} \cdot 1 = \frac{1}{\sqrt{1-x^2}} \\
            &\left(\because \text{By definition, } -\frac{\pi}{2} \le y \le \frac{\pi}{2} \implies \cos y \text{ is positive}\right)
        \end{align*}
        
        Similarly, we can prove following two results:
        
   
    \item $\frac{d}{dx} \left( \cos^{-1} x \right) = \frac{-1}{\sqrt{1 - x^2}}$
    
    \item $\frac{d}{dx} \left( \tan^{-1} x \right) = \frac{1}{1 + x^2}$


\end{enumerate}