


OLD MELODIES

\noindent Differentiation | \textbf{123}

\paragraph{Example 6.} The position of a particle moving along \(x\)-axis varies with time \( t \)
according as 
\[
x = t^2 - t + 1
\]
Velocity \( v_x \) and acceleration \( a_x \) of the particles are defined as
\[
v_x = \frac{dx}{dt} \quad \text{and} \quad a_x = \frac{dv_x}{dt}
\]
(i) Find velocity and acceleration at \( t = 1 \).

(ii) When is the velocity of the particle zero?

\noindent \textbf{Solution.} 
\[
v_x = \frac{dx}{dt} = \frac{d(t^2 - t + 1)}{dt} = 2t - 1
\]

\[
a_x = \frac{dv_x}{dt} = \frac{d(2t - 1)}{dt} = 2
\]

(i) At \( t = 1 \),
\[
v_x = 2 \times 1 - 1 = 1
\]
\[
a_x = 2
\]

(ii) \( v_x = 0 \)
\begin{align*}
\Rightarrow & \quad 2t - 1 = 0 \\
\Rightarrow & \quad t = \frac{1}{2} 
\end{align*}
Hence, \( v_x = 0 \) at \( t = \frac{1}{2} \)

\paragraph{Example 7.} The position of a particle moving in \( xy \)-plane varies with time \( t \)
according as 
\[
x = t + 1, \quad y = t - t^2
\]
Find \(\frac{dy}{dx}\)

\noindent \textbf{Solution.} 
\[
\frac{dy}{dx} = \frac{dy}{dt} \bigg/ \frac{dx}{dt} = \frac{d(t - t^2)}{dt} \bigg/ \frac{d(t + 1)}{dt} = \frac{(1 - 2t)}{1} = 1 - 2t
\]

\paragraph{Example 8.} The velocity \( v_x \) of a particle moving along \( x \)-axis varies with its
position \( x \) according as \( v_x = x^2 + 2x - 4 \)

Find acceleration \( a_x \) of the particle as a function of its position \( x \). Velocity \( v_x \) and acceleration \( a_x \) of the particle are defined as \( v_x = \frac{dx}{dt}, \, a_x = \frac{dv_x}{dt} \) where \( t \) denotes time

\noindent \textbf{Solution.} 
\[
a_x = \frac{dv_x}{dt}
\]
\[
\frac{dv_x}{dx} \cdot \frac{dx}{dt} = v_x \cdot \frac{dv_x}{dx}
\]
\[
a_x = (x^2 + 2x - 4) \cdot \frac{d (x^2 + 2x - 4)}{dx}
\]
\[
a_x = (x^2 + 2x - 4)(2x + 2)
\]
\[
a_x = 2 (x + 1) (x^2 + 2x - 4)
\]

