\vbtitle{\textbf{Illustrations: Circle}}
\BgThispage
\begin{enumerate}
    \item Find the center and radius of the circle with the equation \( x^2 + y^2 - 4x - 6y - 12 = 0 \).
    \begin{solution}
        \begin{align*}
            x^2 + y^2 - 4x - 6y - 12 &= 0 \\
            x^2 - 4x + y^2 - 6y &= 12 \\
            x^2 - 4x + 4 + y^2 - 6y + 9 &= 12 + 4 + 9 \\
            (x - 2)^2 + (y - 3)^2 &= 25
        \end{align*}
        The center of the circle is \( (2, 3) \) and the radius is \( 5 \).
    \end{solution}

    \item Two straight lines \( 3x + 4y - 3 = 0 \) and \( 4x - 3y - 4 = 0 \) intersect at the point \( A \). Find the equation of the circle with \( A \) as the center and \( 5 \) as the radius.
    \begin{solution}
        \begin{align*}
            3x + 4y - 3 &= 0 \\
            4x - 3y - 4 &= 0 \\
            \intertext{Multiplying the first equation by 3 and the second equation by 4, we get}
            9x + 12y - 9 &= 0 \\
            16x - 12y - 16 &= 0 \\
            \intertext{Adding the two equations, we get}
            25x - 25 &= 0 \\
            x &= 1 \\
            \intertext{Substituting the value of \( x \) in the first equation, we get}
            3 + 4y &= 3 \\
            4y &= 0 \\
            y &= 0
        \end{align*}
        The point of intersection of the two lines is \( A(1, 0) \). The equation of the circle is
        \begin{align*}
            (x - 1)^2 + (y - 0)^2 &= 5^2 \\
            (x - 1)^2 + y^2 &= 25 \\
            x^2 - 2x + 1 + y^2 &= 25 \\
            \Aboxed{x^2 + y^2 - 2x - 24 &= 0}
        \end{align*}
    \end{solution}
\end{enumerate}