
\documentclass{article}
\usepackage{amsmath}

\begin{document}

\section*{Solution}

\begin{align*}
(a)\quad & \int_0^1 x dx = \left[ \frac{x^2}{2} \right]_0^1 = \frac{1^2}{2} - \frac{0^2}{2} = \frac{1}{2} \\
(b)\quad & \int_0^{\pi/2} \sin^2 x \cdot \cos x \, dx \\
& \text{Let} \quad y = \sin x \\
& \quad \frac{dy}{dx} = \cos x \\
& \quad dy = \cos x \, dx \\
& \text{When} \quad x = \frac{\pi}{2}, \quad y = 1 \quad \text{and when} \quad x = 0, \quad y = 0. \\
& \text{Hence, on substitution} \\
& \int_0^{\pi/2} \sin^2 x \cos x \, dx = \int_0^1 y^2 \, dy = \left[ \frac{y^3}{3} \right]_0^1 = \frac{1^3}{3} - \frac{0^3}{3} = \frac{1}{3} \\
(c)\quad & \int_1^2 \ln x \, dx = \left[ x \ln x - x \right]_1^2 \\
& = (2 \ln 2 - 2) - (1 \ln 1 - 1) \\
& = 2 \ln 2 - 2 - 0 + 1 = 2 \ln 2 - 1 \quad \left(\because \int_1^a \ln x \, dx = x \ln x - x \right) \\
(d)\quad & \int_{-1}^1 |x| \, dx = \int_{-1}^0 |x| \, dx + \int_0^1 |x| \, dx \quad \left(\because \int_a^b f(x) \, dx = \int_a^c f(x) \, dx + \int_c^b f(x) \, dx \right) \\
& \text{We know that} \\
& |x| = 
\begin{cases} 
x, & x \geq 0 \\
-x, & x < 0 
\end{cases} \\
& \int_{-1}^0 |x| \, dx = \int_{-1}^0 (-x) \, dx \quad (: x \text{ varies from } -1 \text{ to } 0; \, : |x| = -x) \\
& \int_0^1 |x| \, dx = \int_0^1 x \, dx \quad (: x \text{ varies from } 0 \text{ to } 1; \, : |x| = x) \\
& \int_{-1}^1 |x| \, dx = \int_{-1}^0 (-x) \, dx + \int_0^1 x \, dx = \left[ -\frac{x^2}{2} \right]_{-1}^0 + \left[ \frac{x^2}{2} \right]_0^1 \\
& = -\frac{0^2 - (-1)^2}{2} + \frac{1^2 - 0^2}{2} = -\frac{-1}{2} + \frac{1}{2} = 1 \\
(e)\quad & \int_0^{\pi/4} \sqrt{1 - \sin 2x} \, dx = \int_0^{\pi/4} \sqrt{\sin^2 x + \cos^2 x - 2 \sin x \cdot \cos x} \, dx \\
& = \int_0^{\pi/4} \sqrt{(\sin x - \cos x)^2} \, dx = \int_0^{\pi/4} |\sin x - \cos x| \, dx \\
& | \sin x - \cos x | = 
\begin{cases} 
\cos x - \sin x, & 0 \leq x \leq \frac{\pi}{4} \\
\sin x - \cos x, & \frac{\pi}{4} \leq x \leq \frac{\pi}{2} 
\end{cases} \\
& = \int_0^{\pi/4} (\cos x - \sin x) \, dx + \int_{\pi/4}^{\pi/2} (\sin x - \cos x) \, dx \\
& \quad = \left[ \sin x - \cos x \right]_0^{\pi/4} + \left[ \cos x - \sin x \right]_{\pi/4}^{\pi/2} \\
& = (\sin \frac{\pi}{4} - \cos \frac{\pi}{4}) - (0 - 1) + (0 - 1) - (-1) = 0
\end{align*}

\end{document}
