
\documentclass{article}
\usepackage{amsmath}

\begin{document}

\section*{Mathematics For Learning Physics}

\textbf{162}

\[
\begin{aligned}
    \frac{dy}{dx} &= 2 \\
    \Rightarrow \quad \int \frac{dy}{dx} &= \int 2 \\
    \Rightarrow \quad y &= 2x + c
\end{aligned}
\]

On substitution,
\[
\int \frac{dx}{1 + 2x} = \int \frac{dy}{2y} = \frac{1}{2} \ln|2y| = \frac{1}{2} \ln (\sqrt{y}) + c = \sqrt{y} + c = \frac{1}{2} \ln |y|
\]

(d)
\[
\int \sin 2x \, dx = \frac{\cos 2x}{2} + c
\]

\[
\begin{aligned}
\intertext{(e)}
\int \cos^2 x \, dx &= \int \frac{(1 + \cos 2x)}{2} \, dx = \left( \frac{1}{2} \right) \int \, dx + \left( \frac{1}{2} \right) \int \cos 2x \, dx \\
&= \frac{x}{2} + \frac{\sin 2x}{4} + c
\end{aligned}
\]

(f)
\[
\int \sin^2 x \, dx = \int \frac{(1 - \cos 2x)}{2} \, dx = \left( \frac{1}{2} \right) \int \, dx - \left( \frac{1}{2} \right) \int \cos 2x \, dx = \frac{x}{2} - \frac{\sin 2x}{4} + c
\]

(g)
\[
\int \sec x \, \tan x \, dx = \sec x + c
\]

(h)
\[
\begin{aligned}
    \int \csc x (\csc x - 1) \, dx &= \int \csc^2 x \, dx - \int \csc x \, dx \\
    &= -\cot x - \ln (\csc x - \cot x) + c
\end{aligned}
\]

(i)
\[
\begin{aligned}
    \int e^{2x + 3x} \, dx &= \int e^{2x} \, dx + \int e^{-3x} \, dx \\
    &= \frac{e^{2x}}{2} - \frac{e^{-3x}}{3} + c
\end{aligned}
\]

(j)
\[
\begin{aligned}
    \int \cos^2 x \sin x \, dx \\
    \intertext{Let}
    y &= \cos x \\
    \Rightarrow \frac{dy}{dx} &= -\sin x \\
    dy &= -\sin x \, dx \\
    \int \cos^2 x \sin x \, dx &= \int y^2 (-dy) \\
    &= -\int y^2 \, dy \\
    &= -\frac{y^3}{3} + c = -\frac{\cos^3 x}{3} + c
\end{aligned}
\]

(k)
\[
\begin{aligned}
    \int \cos x \sin^n x \, dx \\
    \intertext{Let}
    y &= \sin x \\
    \Rightarrow \frac{dy}{dx} &= \cos x \\
    dy &= \cos x \, dx \\
    \int \cos x \sin^n x \, dx &= \int y^n \, dy = \frac{y^{n+1}}{n+1} + c = \frac{\sin^{n+1} x}{n+1} + c
\end{aligned}
\]

(l)
\[
\begin{aligned}
    \int \sec^2 x \ln (\tan x) \, dx \\
    \intertext{Let}
    y &= \tan x \\
    \Rightarrow dy &= \sec^2 x \, dx \\
    \int \sec^2 x \ln (\tan x) \, dx &= \int \ln y \, dy \quad \left[ \int u \, dv = uv - \int v \, du \right] \\
    &= y \ln y \Big|_{1}^{\sec x} - \int \frac{dy}{y}
\end{aligned}
\]
\[\int \sec^2 x \ln (\tan x) \, dx = y \ln y - \left( \int \frac{dy}{y} \right) (y) \, dy\]
\[
(\ln y)y - \left( \frac{y}{y} - 1 \right) \left( \frac{1}{2} y) \, dy \right)
\]
\[
= y \ln y - y + c = \tan x \ln (\tan x) - \tan x + c
\]

\end{document}
