
\item A radius vector of a point A relative to the origin varies with time \( t \) as \( \mathbf{r} = at\mathbf{i} - bt^3\mathbf{j} \), where \( a \) and \( b \) are positive constants, and \( \mathbf{i} \) and \( \mathbf{j} \) are the unit vectors of the \( x \) and \( y \) axes. Find:
    \begin{enumerate}
        \item the equation of the point's trajectory \( y(x) \); plot this function;
        \item the time dependence of the velocity \( \mathbf{v} \) and acceleration \( \mathbf{w} \) vectors, as well as of the moduli of these quantities;
        \item the time dependence of the angle \( \alpha \) between the vectors \( \mathbf{w} \) and \( \mathbf{v} \);
        \item the mean velocity vector averaged over the first \( t \) seconds of motion, and the modulus of this vector.
    \end{enumerate}

\begin{solution}
    \begin{center}
        \begin{tikzpicture}
            \pic at (0, 0) {frame=3cm};
        \end{tikzpicture}
    \end{center}
    
    \begin{align*}
        \intertext{(a) As}
        \vec{r} &= at\hat{i} - bt^2\hat{j} \\
        \intertext{So,}
        x &= at,\ y = -bt^2 \\
        \intertext{and therefore}
        y &= \dfrac{-bx^2}{a^2}
        \intertext{which is equation of a parabola, whose graph is shown in the figure.}
        \intertext{(b) As}
        \vec{r} &= at\hat{i} - bt^2\hat{j} \\
        \intertext{So,}
        \vec{v} &= \dfrac{d\vec{r}}{dt} = a\hat{i} - 2bt\hat{j} \tag{1} \\
        v &= \sqrt{a^2 + (-2bt)^2} = \sqrt{a^2 + 4b^2t^2}
        \intertext{Differentiating Eq. (1) with respect to time, we get}
        \vec{w} &= \dfrac{d\vec{v}}{dt} = -2b\hat{j} \\
        \intertext{So,}
        |\vec{w}| &= w = 2b \\
        \intertext{(c)}
        \cos{\alpha} &= \dfrac{\vec{v} \cdot \vec{w}}{vw} = \dfrac{(a\hat{i} - 2bt\hat{j}) \cdot (-2b\hat{j})}{(\sqrt{a^2 + 4b^2 t^2}) 2b} \\
        \intertext{or}
        \cos{\alpha} &= \dfrac{2bt}{\sqrt{a^2 + 4b^2 t^2}} \\
        \intertext{So,}
        \tan{\alpha} &= \dfrac{a}{2bt}\ \text{or}\ \alpha = \tan^{-1}\left(\dfrac{a}{2bt}\right)
        \intertext{(d) The mean velocity vector}
        \left<\vec{v}\right> &= \dfrac{\int{\vec{v} dt}}{\int dt} = \dfrac{\int_0^t (a\hat{i} - 2bt\hat{j}) dt}{t} = a\hat{i} - bt\hat{j} \\
        \intertext{Hence,}
        \left<|\vec{v}|\right> &= \sqrt{a^2 + (-bt)^2} = \sqrt{a^2 + b^2 t^2}
    \end{align*}
\end{solution}
