\item A fixed pulley carries a weightless thread with masses $m_{1}$ and $m_{2}$ at its ends. There is friction between the thread and the pulley. It is such that the thread starts slipping when the ratio $m_{2}/m_{1} = \eta_{0}$. Find:
    \begin{enumerate}
        \item the friction coefficient;
        \item the acceleration of the masses when $m_{2}/m_{1} = \eta > \eta_{0}$.
    \end{enumerate}
\begin{solution}
    \begin{center}
        \begin{tikzpicture}
            \pic at (0, 0) {frame=3cm};
        \end{tikzpicture}
    \end{center}
    
    \begin{align*}
        \intertext{Applying Newton's second law of motion in projection form, $F_n = mw_n$ for this element,}
        (T + dT) \sin (d\theta/2) + T \sin (d\theta/2) - dN &= dm\omega^2R = 0\\
        \intertext{or}
        2T \sin (d\theta/2) &= dN \quad [\text{neglecting the term } (dT \sin d\theta/2)]\\
        \intertext{or}
        T \, d\theta &= dN \left( \text{as } \sin \dfrac{d\theta}{2} \approx \dfrac{d\theta}{2} \right) \tag{1}\\
        \intertext{Also,}
        dfr &= kdN = (T + dT) - T = dT \tag{2}\\
        \intertext{From Eqs. (1) and (2)}
        kT \, d\theta &= dT \quad \text{or} \quad \dfrac{dT}{T} = kd\theta \\
        \intertext{Integrating $\theta \text{ from } 0 \text{ to } \theta = \pi$, we get}
        \ln \dfrac{T_2}{T_1} &= k\pi \tag{3}\\
        \intertext{So,}
        k &= \dfrac{1}{\pi} \ln \dfrac{T_2}{T_1} = \dfrac{1}{\pi} \ln \eta_0\\
        \left( \dfrac{T_2}{T_1} = \dfrac{m_2g}{m_1g} = \dfrac{m_2}{m_1} = \eta_0 \right)\\
        \intertext{When $m_2/m_1 = \eta > \eta_0$, the blocks will move with the same value of acceleration (say $w$) and clearly $m_2$ moves downward. From Newton's second law in projection form (downward for $m_2$ and upward for $m_1$), we get}
        m_2g - T_2 &= m_2w \tag{4}\\
        T_2 - m_1g &= m_1w \tag{5}\\
        \intertext{Also}
        \dfrac{T_2}{T_1} &= \eta_0 \tag{6}\\
        \intertext{Simultaneous solution of Eqs. (4), (5), and (6) yields}
        w &= \dfrac{(m_2 - \eta_0 m_1) g}{(m_2 + \eta_0 m_1)} = \dfrac{(\eta - \eta_0)}{(\eta + \eta_0)} g \quad \left( \dfrac{m_2}{m_1} = \eta \right)
    \end{align*}
\end{solution}
